state/Compiler.fst
@@ -43,13 +43,13 @@ let src_language1 : language (st_wp int) = {
 
 noeq
 type tgt_interface1 = {
-  ct : inv : (heap -> Type0) -> prref: ref_pred -> hrel : FStar.Preorder.preorder heap -> Type u#a;
+  ct : inv : (heap -> Type0) -> prref: mref_pred -> hrel : FStar.Preorder.preorder heap -> Type u#a;
   ct_targetlang : targetlang default_spec (ct (Mktuple3?._1 default_spec) (Mktuple3?._2 default_spec) (Mktuple3?._3 default_spec));
 }
 
 type ctx_tgt1 (i:tgt_interface1) = 
   inv  : (heap -> Type0) -> 
-  prref: ref_pred ->
+  prref: mref_pred ->
   (** ^ if this predicate would be also over heaps, then the contexts needs witness&recall in HO settings **)
   hrel : FStar.Preorder.preorder heap ->
   read :  ((#t:shareable_typ) -> r:ref (to_Type t) -> 
@@ -69,116 +69,6 @@ type ctx_tgt1 (i:tgt_interface1) =
 type prog_tgt1 (i:tgt_interface1) = i.ct (Mktuple3?._1 default_spec) (Mktuple3?._2 default_spec) (Mktuple3?._3 default_spec) -> SST int (fun _ -> True) (fun _ _ _ -> True)
 type whole_tgt1 = (unit -> SST int (fun _ -> True) (fun _ _ _ -> True))
 
-
-let rec lemma_forall_refs_heap_forall_refs_witnessed #t (v:to_Type t) (pred:ref_heap_stable_pred) :
-  ST unit 
-    (requires (fun h0 -> forall_refs_heap pred h0 v))
-    (ensures (fun h0 _ h1 -> h0 == h1 /\ forall_refs (fun r -> witnessed (pred r)) v)) =
-  match t with
-  | SUnit -> ()
-  | SNat -> ()
-  | SSum t1 t2 -> begin
-    let v : either (to_Type t1) (to_Type t2) = v in
-    match v with
-    | Inl v' -> lemma_forall_refs_heap_forall_refs_witnessed v' pred
-    | Inr v' -> lemma_forall_refs_heap_forall_refs_witnessed v' pred
-  end
-  | SPair t1 t2 -> 
-    let v : (to_Type t1) * (to_Type t2) = v in
-    lemma_forall_refs_heap_forall_refs_witnessed (fst v) pred;
-    lemma_forall_refs_heap_forall_refs_witnessed (snd v) pred
-  | SRef t' ->
-    let v : ref (to_Type t') = v in 
-    witness (pred v);
-    ()
-  | SLList t' -> begin
-    let v : linkedList (to_Type t') = v in
-    match v with
-    | LLNil -> ()
-    | LLCons v xsref ->
-      lemma_forall_refs_heap_forall_refs_witnessed v pred;
-      witness (pred xsref)
-  end
-
-let rec lemma_forall_refs_witnessed_forall_refs_heap #t (v:to_Type t) (pred:ref_heap_stable_pred) :
-  ST unit 
-    (requires (fun _ -> forall_refs (fun r -> witnessed (pred r)) v))
-    (ensures (fun h0 _ h1 -> h0 == h1 /\ forall_refs_heap pred h1 v)) =
-  match t with
-  | SUnit -> ()
-  | SNat -> ()
-  | SSum t1 t2 -> begin
-    let v : either (to_Type t1) (to_Type t2) = v in
-    match v with
-    | Inl v' -> lemma_forall_refs_witnessed_forall_refs_heap v' pred
-    | Inr v' -> lemma_forall_refs_witnessed_forall_refs_heap v' pred
-  end
-  | SPair t1 t2 -> 
-    let v : (to_Type t1) * (to_Type t2) = v in
-    lemma_forall_refs_witnessed_forall_refs_heap (fst v) pred;
-    lemma_forall_refs_witnessed_forall_refs_heap (snd v) pred
-  | SRef t' ->
-    let v : ref (to_Type t') = v in 
-    recall (pred v);
-    ()
-  | SLList t' -> begin
-    let v : linkedList (to_Type t') = v in
-    match v with
-    | LLNil -> ()
-    | LLCons v xsref ->
-      lemma_forall_refs_witnessed_forall_refs_heap v pred;
-      recall (pred xsref)
-  end
-
-let rec lemma_forall_refs_join #t (v:to_Type t) (pred1 pred2:ref_pred) :
-  Lemma (requires (forall_refs pred1 v /\ forall_refs pred2 v))
-        (ensures (forall_refs (fun r -> pred1 r /\ pred2 r) v)) =
-  match t with
-  | SUnit -> ()
-  | SNat -> ()
-  | SSum t1 t2 -> begin
-    let v : either (to_Type t1) (to_Type t2) = v in
-    match v with
-    | Inl v' -> lemma_forall_refs_join v' pred1 pred2
-    | Inr v' -> lemma_forall_refs_join v' pred1 pred2
-  end
-  | SPair t1 t2 -> 
-    let v : (to_Type t1) * (to_Type t2) = v in
-    lemma_forall_refs_join (fst v) pred1 pred2;
-    lemma_forall_refs_join (snd v) pred1 pred2
-  | SRef t' -> ()
-  | SLList t' -> begin
-    let v : linkedList (to_Type t') = v in
-    match v with
-    | LLNil -> ()
-    | LLCons v xsref ->
-      lemma_forall_refs_join v pred1 pred2
-  end
-
-let rec lemma_forall_refs_split #t (v:to_Type t) (pred1 pred2:ref_pred) :
-  Lemma (requires (forall_refs (fun r -> pred1 r /\ pred2 r) v))
-        (ensures (forall_refs pred1 v /\ forall_refs pred2 v)) =
-  match t with
-  | SUnit -> ()
-  | SNat -> ()
-  | SSum t1 t2 -> begin
-    let v : either (to_Type t1) (to_Type t2) = v in
-    match v with
-    | Inl v' -> lemma_forall_refs_split v' pred1 pred2
-    | Inr v' -> lemma_forall_refs_split v' pred1 pred2
-  end
-  | SPair t1 t2 -> 
-    let v : (to_Type t1) * (to_Type t2) = v in
-    lemma_forall_refs_split (fst v) pred1 pred2;
-    lemma_forall_refs_split (snd v) pred1 pred2
-  | SRef t' -> ()
-  | SLList t' -> begin
-    let v : linkedList (to_Type t') = v in
-    match v with
-    | LLNil -> ()
-    | LLCons v xsref ->
-      lemma_forall_refs_split v pred1 pred2
-  end
 
 
 #push-options "--split_queries always"
